added test vectors for HKDF

providers/test/Test.Vectors.fst
@@ -192,6 +192,64 @@ let hmac_vectors_tmp = List.Tot.map (fun h ->
 
 
 
+/// HKDF
+/// https://tools.ietf.org/html/rfc5869.html
+/// pls extend me! We miss SHA384 and SHA512 tests
+///
+/// The test is in 2 steps:
+/// prk <- extract sal ikm        
+/// okm <- expand prk info okmlen 
+
+noeq noextract
+type hkdf_vector = {
+  ha:   hash_alg;
+  ikm:  hex_encoded;  // input key materials
+  salt: hex_encoded; // input salt 
+  info: hex_encoded; // expansion label
+  prk:  hex_encoded;  // extracted pseudo-random key (its length is tagLen ha)
+  okm:  hex_encoded;  // output: expanded key materials (its length is an input)
+}
+
+noextract 
+let hkdf_vectors = [{
+    // Test Case 1
+    // Basic test case with SHA-256
+    ha   = SHA256;
+    ikm  = h"0b0b0b0b0b0b0b0b0b0b0b0b0b0b0b0b0b0b0b0b0b0b";// (22 octets)
+    salt = h"000102030405060708090a0b0c";// (13 octets)
+    info = h"f0f1f2f3f4f5f6f7f8f9";// (10 octets)
+    prk  = h"077709362c2e32df0ddc3f0dc47bba6390b6c73bb50f9c3122ec844ad7c2b3e5";// (32 octets)
+    okm  = h"3cb25f25faacd57a90434f64d0362f2a2d2d0a90cf1a5a4c5db02d56ecc4c5bf34007208d5b887185865";// (42 octets)
+  }; {
+    // Test Case 2
+    // Test with SHA-256 and longer inputs/outputs
+    ha   = SHA256;
+    ikm  = h"000102030405060708090a0b0c0d0e0f101112131415161718191a1b1c1d1e1f202122232425262728292a2b2c2d2e2f303132333435363738393a3b3c3d3e3f404142434445464748494a4b4c4d4e4f";// (80 octets)
+    salt = h"606162636465666768696a6b6c6d6e6f707172737475767778797a7b7c7d7e7f808182838485868788898a8b8c8d8e8f909192939495969798999a9b9c9d9e9fa0a1a2a3a4a5a6a7a8a9aaabacadaeaf";// (80 octets)
+    info = h"b0b1b2b3b4b5b6b7b8b9babbbcbdbebfc0c1c2c3c4c5c6c7c8c9cacbcccdcecfd0d1d2d3d4d5d6d7d8d9dadbdcdddedfe0e1e2e3e4e5e6e7e8e9eaebecedeeeff0f1f2f3f4f5f6f7f8f9fafbfcfdfeff";// (80 octets)
+    prk  = h"06a6b88c5853361a06104c9ceb35b45cef760014904671014a193f40c15fc244";// (32 octets)
+    okm  = h"b11e398dc80327a1c8e7f78c596a49344f012eda2d4efad8a050cc4c19afa97c59045a99cac7827271cb41c65e590e09da3275600c2f09b8367793a9aca3db71cc30c58179ec3e87c14c01d5c1f3434f1d87";// (82 octets)
+  }; {
+    // Test Case 3
+    // Test with SHA-256 and zero-length salt/info
+    ha   = SHA256;
+    ikm  = h"0b0b0b0b0b0b0b0b0b0b0b0b0b0b0b0b0b0b0b0b0b0b";// (22 octets)
+    salt = h"";
+    info = h"";
+    prk  = h"19ef24a32c717b167f33a91d6f648bdf96596776afdb6377ac434c1c293ccb04";// (32 octets)
+    okm  = h"8da4e775a563c18f715f802a063c5a31b8a11f5c5ee1879ec3454e5f3c738d2d9d201395faa4b61a96c8";// (42 octets)
+  }]
+
+noextract
+let hkdf_vectors_tmp = List.Tot.map (fun h ->
+  h.ha, h.ikm, h.salt, h.info, h.prk, h.okm
+) hkdf_vectors
+
+%splice[] (lowstarize_toplevel "hkdf_vectors_tmp" "hkdf_vectors_low")
+
+//TODO add test_hkdf, test_hkdf_one as for HMAC
+
+
 /// Cipher block function
 
 type block_cipher =
